Suppose the demand for Wheat is given by the equation$$d_t=a-\gamma p_t$$where $p_t$ is the market price of wheat. The supply equation is given by $$s_t=b+\beta p_t^*+\epsilon_t$$where $p^*_t$ is the farmers expected price of wheat at $t$. The long run equilibrium condition is given by $$s_t=p_t$$Suppose that in time $t$, a negative supply shock occurs that increase $p_t$.
In time $t+1$,  the expected price with [[DAD-DAS framework#Adaptive expectations|adaptive expectations]] is $p_t$. However this price was higher than the equilibrium. Therefore the supply $s_{t+1}$ is higher than equilibrium. Thus the price falls in the next period. The price oscillates between below and above the LR equilibrium till it reaches there again. Graphically, 
![[Pasted image 20240201194439.png|400]]

In order to determine the nature of the effect of the shocks on prices, we can use [[Time Series]] analysis to determine if the series in convergent to the LR equilibrium.

Due to adaptive expectations, $$p_t^*=p_{t-1}$$From the LR equilibrium condition, $$a-\gamma p_t=b+\beta p_t^*+\epsilon_t$$Combining these two, $$a-\gamma p_t=b+\beta p_{t-1}+\epsilon_t$$$$p_t=\frac{a-b}{\gamma}-\frac{\beta}{\gamma}p_{t-1}-\frac{\epsilon_t}{\gamma}$$This is a first order [[Difference equations|difference equation]]. Finding the [[Difference equations#Homogenous solution|homogenous solution]],$$p_t^h=\frac{-\beta}{\gamma}p_{t-1}$$$$p_t^h+\frac{\beta}{\gamma}p_{t-1}=0$$Replacing $p_t$ terms with $A\alpha^t$,$$A\alpha^t+\frac\beta\gamma A\alpha^{t-1}=0$$$$\alpha+\frac\beta\gamma=0$$$$\alpha=\frac{-\beta}\gamma$$Therefore, $$p_t^h=A(\frac{-\beta}\gamma)^t$$Finding the particular solution,
$$p_t=\frac{a-b}{\gamma}-\frac{\beta}{\gamma}p_{t-1}-\frac{\epsilon_t}{\gamma}$$Using backwards iteration, $$p_t=\frac{a-b}{\gamma}-\frac{\beta}{\gamma}(\frac{a-b}{\gamma}-\frac{\beta}{\gamma}p_{t-2}-\frac{\epsilon_{t-1}}{\gamma})-\frac{\epsilon_t}{\gamma}$$$$=\frac{a-b}{\gamma}-\frac{\beta}{\gamma}(\frac{a-b}{\gamma})+(\frac{\beta}{\gamma})^2p_{t-2}+\frac\beta\gamma\frac{\epsilon_{t-1}}{\gamma}-\frac{\epsilon_t}{\gamma}$$$$=\frac{a-b}{\gamma}-\frac{\beta}{\gamma}(\frac{a-b}{\gamma})+(\frac{\beta}{\gamma})^2(\frac{a-b}{\gamma}-\frac{\beta}{\gamma}p_{t-3}-\frac{\epsilon_{t-2}}{\gamma})+\frac\beta\gamma\frac{\epsilon_{t-1}}{\gamma}-\frac{\epsilon_t}{\gamma}$$$$=\frac{a-b}{\gamma}[1+\frac{-\beta}{\gamma}+(\frac{-\beta}{\gamma})^2]+(\frac{-\beta}{\gamma})^3p_{t-3}-\frac1\gamma[\epsilon_t+\frac{-\beta}{\gamma}\epsilon_{t-1}+(\frac{-\beta}\gamma)^2\epsilon_{t-2}]$$
Therefore, $$p_t=\frac{a-b}\gamma\sum_{i=0}^n[(\frac{-\beta}\gamma)^i]+(\frac{-\beta}\gamma)^np_{t-n}-\frac1\gamma\sum_{i=0}^n[(\frac{-\beta}\gamma)^i\epsilon_{t-i}]$$If we assume that $|\frac\beta\gamma|<0$ and $t\to\infty, n\to\infty$,$$p_t=\frac{a-b}\gamma(\frac1{1-(-\beta/\gamma)})+0-\frac1\gamma\sum_{i=0}^n[(\frac{-\beta}\gamma)^i\epsilon_{t-i}]$$$$=\frac{a-b}\gamma(\frac\gamma{\gamma+\beta})-\frac1\gamma\sum_{i=0}^n[(\frac{-\beta}\gamma)^i\epsilon_{t-i}]$$$$p_t^p=\frac{a-b}{\gamma+\beta}-\frac1\gamma\sum_{i=0}^n[(\frac{-\beta}\gamma)^i\epsilon_{t-i}]$$
Finding the general solution, $$p_t=A(\frac{-\beta}\gamma)^t+\frac{a-b}{\gamma+\beta}-\frac1\gamma\sum_{i=0}^n[(\frac{-\beta}\gamma)^i\epsilon_{t-i}]$$We need to find the value of the arbitrary constant $A$. Therefore, if the initial condition $p_0$ is given, $$p_0=A(\frac{-\beta}\gamma)^0+\frac{a-b}{\gamma+\beta}-\frac1\gamma\sum_{i=0}^n[(\frac{-\beta}\gamma)^i\epsilon_{t-i}]$$$$A=p_0-\frac{a-b}{\gamma+\beta}+\frac1\gamma\sum_{i=0}^n[(\frac{-\beta}\gamma)^i\epsilon_{t-i}]$$Substituting this into the general solution equation, $$p_t=[p_0-\frac{a-b}{\gamma+\beta}+\frac1\gamma\sum_{i=0}^n((\frac{-\beta}\gamma)^i\epsilon_{t-i})](\frac{-\beta}\gamma)^t+\frac{a-b}{\gamma+\beta}-\frac1\gamma\sum_{i=0}^n[(\frac{-\beta}\gamma)^i\epsilon_{t-i}]$$
### Finding the impulse response function
A function that shows how the entire time path is effected by stochastic shocks. Found by taking derivatives of the timepath with respect to the disturbance terms. $$\frac{\partial p_t}{\partial\epsilon_t}=-\frac{1}{\gamma}$$$$\frac{\partial p_{t+1}}{\partial\epsilon_t}=-\frac{1}{\gamma}(\frac{-\beta}\gamma)$$$$\frac{\partial p_{t+2}}{\partial\epsilon_t}=-\frac{1}{\gamma}(\frac{-\beta}\gamma)^2$$$$\frac{\partial p_{t+n}}{\partial\epsilon_t}=-\frac{1}{\gamma}(\frac{-\beta}\gamma)^n$$Which is the impulse response function. As $|\beta/\gamma|<1$, the effect of the shock dies down over time and the series converges to its long run equilibrium.